ADTExamples/MinPlusMax.v
@@ -1,0 +1,152 @@
+Require Import Common String ADT ADTRefinement.Specs.
+Require Import ADTRefinement ADTCache ADTRepInv Pick ADTHide DelegateMethods.
+Require Import ADTExamples.BinaryOperationSpec ADTExamples.CombineBinaryOperationsSpec.
+
+Section MinMaxExample.
+
+  Definition MinMaxSig : ADTSig :=
+    ADTsignature {
+        "Insert" : rep ✕ nat → rep ;
+        "Min" : rep ✕ nat → nat ,
+        "Max" : rep ✕ nat → nat
+      }%ADTSig.
+
+  Definition defaultSpec : nat -> Prop := fun _ => True.
+
+  Definition MinMaxSpec 
+  : ADT MinMaxSig :=
+    ADTRep multiset `[
+             def "Insert" `[ m `: rep , n `: nat ]` : rep :=
+               {m' | add_spec m n m'}%comp ;
+             def "Min" `[m `: rep , n `: nat ]` : nat :=
+                 {n' | bin_op_spec le defaultSpec m n n'}%comp ,
+             def "Max" `[m `: rep , n `: nat ]` : nat :=
+                 {n' | bin_op_spec ge defaultSpec m n n'}%comp
+           ]`%ADT .
+
+  Variable MinMaxImpl : ADT MinMaxSig.
+  Variable refineMinMax : refineADT MinMaxSpec MinMaxImpl.
+
+  Definition foo idx : 
+    fst (ObserverDomCod (CombTwoOpCollectionSig "MinPlusMax") idx) -> 
+    nat.
+  Proof.
+    destruct idx; inversion s_bounded.
+    simpl.
+    caseEq (obsSig_eq ("MinPlusMax" : rep ✕ nat → nat) bounded_s); eauto.
+    elimtype False.
+    inversion sbound; simpl in *; subst.
+    unfold obsSig_eq in H; find_if_inside; eauto; discriminate.
+    eauto.
+  Defined.
+
+  Definition bar idx : 
+    nat -> 
+    snd (ObserverDomCod (CombTwoOpCollectionSig "MinPlusMax") idx).
+  Proof.
+    destruct idx; inversion s_bounded.
+    simpl.
+    caseEq (obsSig_eq ("MinPlusMax" : rep ✕ nat → nat) bounded_s); eauto.
+    elimtype False.
+    inversion sbound; simpl in *; subst.
+    unfold obsSig_eq in H; find_if_inside; eauto; discriminate.
+    eauto.
+  Defined.
+
+  Definition MinPlusMaxImpl (defaultValue : nat)
+  : Sharpened MinPlusMaxSpec.
+  Proof.
+    eapply SharpenStep.
+    eapply refineADT_DelegatedMethods with 
+    (delegateDomCod := ObserverDomCod MinMaxSig)
+    (delegateADT := MinMaxImpl).
+    eapply SharpenStep with (adt' := 
+                               {|
+     Rep := Rep MinPlusMaxSpec * Rep MinMaxImpl;
+     MutatorMethods := fun
+                         (idx : MutatorIndex
+                                  (CombTwoOpCollectionSig "MinPlusMax"))
+                         (r : Rep MinPlusMaxSpec * Rep MinMaxImpl)
+                         (x : MutatorDom
+                                (CombTwoOpCollectionSig "MinPlusMax") idx) =>
+                       r1 <- MutatorMethods MinPlusMaxSpec idx (fst r) x;
+                       r2 <- MutatorMethods MinMaxImpl idx (snd r) x;
+                       ret (r1, r2);
+     ObserverMethods := fun
+                          (idx : ObserverIndex
+                                   (CombTwoOpCollectionSig "MinPlusMax"))
+                          (r : Rep MinPlusMaxSpec * Rep MinMaxImpl) 
+                          n =>
+                         (min <- (ObserverMethods MinMaxImpl
+                                                  {|bounded_s := "Min"%string |} (snd r) (foo _ n));
+                          max <- (ObserverMethods MinMaxImpl
+                                                  {|bounded_s := "Max"%string |} (snd r) (foo _ n));
+                          ret (bar idx (min + max)))%comp |}).
+    assert (exists SiR : multiset -> Rep MinMaxImpl -> Prop,
+              (forall idx : ObserverIndex MinMaxSig,
+                refineObserver SiR (ObserverMethods MinMaxSpec idx)
+                               (ObserverMethods MinMaxImpl idx)) /\
+              (forall idx : MutatorIndex MinMaxSig,
+                  refineMutator SiR (MutatorMethods MinMaxSpec idx)
+                                 (MutatorMethods MinMaxImpl idx))).
+    inversion refineMinMax; eauto.
+    clear refineMinMax; destruct H as [SiR [refineMinMaxObs refineMinMaxMut] ].
+    eapply refineADT_Build_ADT_Rep with 
+    (SiR := fun (or nr : Rep MinPlusMaxSpec * Rep MinMaxImpl) => 
+              or = nr /\
+              SiR (fst nr) (snd nr)).
+    - intro.
+      assert (exists pf,
+                mutIdx = {| bounded_s := "Insert"%string;
+                            s_bounded := pf |}) as mutIdx_eq by 
+          (clear;
+           destruct mutIdx; destruct s_bounded; inversion sbound; 
+           subst; simpl; 
+           [ exists {| sbound := sbound |}; reflexivity
+                  | inversion H ]) ;
+      destruct mutIdx_eq as [pf mutIdx_eq]; rewrite mutIdx_eq.
+      unfold refineMutator; intros; intuition; subst.
+      unfold refine; intros; econstructor; eauto.
+      econstructor; split; eauto.
+      inversion_by computes_to_inv; subst; simpl.
+      generalize (refineMinMaxMut _  _ _ n H1 _ H2); intros.
+      inversion_by computes_to_inv.
+      unfold getMutDef in H0, H3; simpl in H0, H3.
+      inversion_by computes_to_inv.
+      unfold add_spec in *.
+      assert (x1 = x) by 
+          (apply functional_extensionality;
+           intros; rewrite H0, H3; reflexivity).
+      rewrite H in H4; assumption.
+    - intro; 
+      assert (exists pf,
+                 obsIdx = {| bounded_s := "MinPlusMax"%string;
+                            s_bounded := pf |}) as obsIdx_eq by 
+          (clear;
+           destruct obsIdx; destruct s_bounded; inversion sbound; 
+           subst; simpl; 
+           [ exists {| sbound := sbound |}; reflexivity
+                  | inversion H ]) ;
+      destruct obsIdx_eq as [pf obsIdx_eq]; rewrite obsIdx_eq.
+      simpl; intros; intuition; subst; unfold getObsDef; simpl.
+      unfold two_op_spec, refine; intros.
+      apply computes_to_inv in H; destruct_ex; intuition.
+      apply computes_to_inv in H2; destruct_ex; intuition.
+      apply computes_to_inv in H3; destruct_ex; intuition.
+      destruct pf; subst.
+      econstructor; eexists x; split; eauto.
+      generalize (refineMinMaxObs {|bounded_s := "Min" |} _ _ _ H1 _ H0).
+      simpl; unfold getObsDef; simpl; intros; inversion_by computes_to_inv; eauto.
+      eexists x0; split; eauto.
+      generalize (refineMinMaxObs {|bounded_s := "Max" |} _ _ _ H1 _ H2).
+      simpl; unfold getObsDef; simpl; intros; inversion_by computes_to_inv; eauto.
+    - finish sharpening.
+  Defined.
+
+  (* Show the term derived above as a sanity check. *)
+  Goal (forall b, ObserverMethods (proj1_sig (MinPlusMaxImpl 0)) 
+                                 {| bounded_s := "MinPlusMax" |} = b).
+    simpl.
+  Abort.
+
+End MinMaxExample.
